Started clean up repo

Monad_Play Around/DNFP/Dutch_National_Flag_Monad.thy
@@ -4,7 +4,9 @@ imports
 begin
 
 section\<open>DNFP\<close>
-text\<open>A version using a state monad for storing the list/array that is being sorted\<close>
+text\<open>A version using a state monad for storing the array and the intermediate variable.
+This function takes a parameter that defines the size of the unsorted array (the difference between high and i).
+This makes the recursion well-defined and will ensure termination since loop_update_action decreases the difference for every single call\<close>
 fun dnfp_mon:: "nat \<Rightarrow> (env, unit) state" where
   case0:"dnfp_mon 0  = skip"|
   caseN:"dnfp_mon (Suc n) = do {
@@ -16,427 +18,8 @@ fun dnfp_mon:: "nat \<Rightarrow> (env, unit) state" where
                        else skip
                       )}"
 
-section\<open>Lemmas\<close>
-subsection\<open>Hoare proofs\<close>
-subsection\<open>DNFP_Mon Auxillary lemmas\<close>
-lemma dnfp_aux1: "spec (\<lambda>y. length (xs e) = length (xs y)) (dnfp_mon v) (\<lambda>x y. length (xs e) = length (xs y))"
-  apply(induction v rule: dnfp_mon.induct)
-    apply(simp add: spec_def)
-    apply (simp add: skip_def)
-  apply(simp only: caseN)
-  apply(intro get_rule; intro allI; clarify)
-  apply(intro cond_rule)
-  apply(simp add: loop_update_action_def)
-  apply(intro get_rule; intro allI; clarify)
-  apply(intro seq_rule[of _ _ "(\<lambda>x y. length (xs e) = length (xs y))"])
-  apply(intro cond_rule)
-  apply(simp add: inc_lowbound_def)
-   apply(intro get_rule; intro allI; simp)
-  apply(intro seq_rule[of _ _ "(\<lambda>x y. length (xs e) = length (xs y))"])
-    apply(simp add: spec_def put_def xs_Env_def swap_def put_state_def get_state_def)
-   apply(intro allI; simp)
-   apply(intro get_rule; intro allI)
-  apply(intro seq_rule[of _ _ "(\<lambda>x y. length (xs e) = length (xs y))"])
-    apply(simp add: spec_def put_def i_Env_def put_state_def get_state_def)
-   apply(intro allI; simp)
-         apply(intro get_rule; intro allI)
-    apply(simp add: spec_def put_def low_Env_def put_state_def get_state_def)
-  apply(simp add: dec_highbound_def)
-   apply(intro get_rule; intro allI; simp)
-  apply(intro seq_rule[of _ _ "(\<lambda>x y. length (xs e) = length (xs y))"])
-    apply(simp add: spec_def put_def high_Env_def put_state_def get_state_def)
-   apply(intro allI; simp)
-  apply(intro get_rule; intro allI; simp)
-    apply(simp add: spec_def put_def xs_Env_def swap_def put_state_def get_state_def)
-  apply(simp add: inc_index_def)
-  apply(intro get_rule; intro allI; simp)
-    apply(simp add: spec_def put_def i_Env_def put_state_def get_state_def)
-   apply blast
-    apply(simp add: spec_def put_def i_Env_def put_state_def get_state_def run_state_def)
-  by (simp add: skip_def)
-
-lemma dnfp_aux2: "spec (\<lambda>y. high y \<le> high e) (dnfp_mon v) (\<lambda>x y. high y \<le> high e)"
-  apply(induction v rule: dnfp_mon.induct)
-    apply(simp add: spec_def)
-    apply (simp add: skip_def)
-  apply(simp only: caseN)
-  apply(intro get_rule; intro allI; clarify)
-  apply(intro cond_rule)
-  apply(simp add: loop_update_action_def)
-  apply(intro get_rule; intro allI; clarify)
-  apply(intro seq_rule[of _ _ "(\<lambda>x y. high y \<le> high e)"])
-  apply(intro cond_rule)
-  apply(simp add: inc_lowbound_def)
-   apply(intro get_rule; intro allI; simp)
-  apply(intro seq_rule[of _ _ "(\<lambda>x y. high y \<le> high e)"])
-    apply(simp add: spec_def put_def xs_Env_def swap_def put_state_def get_state_def)
-   apply(intro allI; simp)
-   apply(intro get_rule; intro allI)
-  apply(intro seq_rule[of _ _ "(\<lambda>x y. high y \<le> high e)"])
-    apply(simp add: spec_def put_def i_Env_def put_state_def get_state_def)
-   apply(intro allI; simp)
-         apply(intro get_rule; intro allI)
-    apply(simp add: spec_def put_def low_Env_def put_state_def get_state_def)
-  apply(simp add: dec_highbound_def)
-   apply(intro get_rule; intro allI; simp)
-  apply(intro seq_rule[of _ _ "(\<lambda>x y. high y \<le> high e)"])
-      apply(simp add: spec_def put_def high_Env_def put_state_def get_state_def)
-  apply linarith
-   apply(intro allI; simp)
-  apply(intro get_rule; intro allI; simp)
-    apply(simp add: spec_def put_def xs_Env_def swap_def put_state_def get_state_def)
-  apply(simp add: inc_index_def)
-  apply(intro get_rule; intro allI; simp)
-    apply(simp add: spec_def put_def i_Env_def put_state_def get_state_def)
-   apply blast
-    apply(simp add: spec_def put_def i_Env_def put_state_def get_state_def run_state_def)
-  by (simp add: skip_def)
-
-lemma dnfp_aux3: "spec (\<lambda>y. low e \<le> low y) (dnfp_mon v) (\<lambda>x y. low e \<le> low y)"
-  apply(induction v rule: dnfp_mon.induct)
-    apply(simp add: spec_def)
-    apply (simp add: skip_def)
-  apply(simp only: caseN)
-  apply(intro get_rule; intro allI; clarify)
-  apply(intro cond_rule)
-  apply(simp add: loop_update_action_def)
-  apply(intro get_rule; intro allI; clarify)
-  apply(intro seq_rule[of _ _ "(\<lambda>x y. low e \<le> low y)"])
-  apply(intro cond_rule)
-  apply(simp add: inc_lowbound_def)
-   apply(intro get_rule; intro allI; simp)
-  apply(intro seq_rule[of _ _ "(\<lambda>x y. low e \<le> low y)"])
-    apply(simp add: spec_def put_def xs_Env_def swap_def put_state_def get_state_def)
-   apply(intro allI; simp)
-   apply(intro get_rule; intro allI)
-  apply(intro seq_rule[of _ _ "(\<lambda>x y. low e \<le> low y)"])
-    apply(simp add: spec_def put_def i_Env_def put_state_def get_state_def)
-   apply(intro allI; simp)
-         apply(intro get_rule; intro allI)
-    apply(simp add: spec_def put_def low_Env_def put_state_def get_state_def)
-  apply(simp add: dec_highbound_def)
-   apply(intro get_rule; intro allI; simp)
-  apply(intro seq_rule[of _ _ "(\<lambda>x y. low e \<le> low y)"])
-      apply(simp add: spec_def put_def high_Env_def put_state_def get_state_def)
-   apply(intro allI; simp)
-  apply(intro get_rule; intro allI; simp)
-    apply(simp add: spec_def put_def xs_Env_def swap_def put_state_def get_state_def)
-  apply(simp add: inc_index_def)
-  apply(intro get_rule; intro allI; simp)
-    apply(simp add: spec_def put_def i_Env_def put_state_def get_state_def)
-   apply blast
-    apply(simp add: spec_def put_def i_Env_def put_state_def get_state_def run_state_def)
-  by (simp add: skip_def)
-
-lemma dnfp_aux4: "spec (\<lambda>y. i e \<le> i y) (dnfp_mon v) (\<lambda>x y. i e \<le> i y)"
-  apply(induction v rule: dnfp_mon.induct)
-    apply(simp add: spec_def)
-    apply (simp add: skip_def)
-  apply(simp only: caseN)
-  apply(intro get_rule; intro allI; clarify)
-  apply(intro cond_rule)
-  apply(simp add: loop_update_action_def)
-  apply(intro get_rule; intro allI; clarify)
-  apply(intro seq_rule[of _ _ "(\<lambda>x y. i e \<le> i y)"])
-  apply(intro cond_rule)
-  apply(simp add: inc_lowbound_def)
-   apply(intro get_rule; intro allI; simp)
-  apply(intro seq_rule[of _ _ "(\<lambda>x y. i e \<le> i y)"])
-    apply(simp add: spec_def put_def xs_Env_def swap_def put_state_def get_state_def)
-   apply(intro allI; simp)
-   apply(intro get_rule; intro allI)
-  apply(intro seq_rule[of _ _ "(\<lambda>x y. i e \<le> i y)"])
-    apply(simp add: spec_def put_def i_Env_def put_state_def get_state_def)
-   apply(intro allI; simp)
-         apply(intro get_rule; intro allI)
-    apply(simp add: spec_def put_def low_Env_def put_state_def get_state_def)
-  apply(simp add: dec_highbound_def)
-   apply(intro get_rule; intro allI; simp)
-  apply(intro seq_rule[of _ _ "(\<lambda>x y. i e \<le> i y)"])
-      apply(simp add: spec_def put_def high_Env_def put_state_def get_state_def)
-   apply(intro allI; simp)
-  apply(intro get_rule; intro allI; simp)
-    apply(simp add: spec_def put_def xs_Env_def swap_def put_state_def get_state_def)
-  apply(simp add: inc_index_def)
-  apply(intro get_rule; intro allI; simp)
-    apply(simp add: spec_def put_def i_Env_def put_state_def get_state_def)
-   apply blast
-    apply(simp add: spec_def)
-  by (simp add: skip_def)
-
-lemma dnfp_aux5: "spec (\<lambda>y. high y - i y \<le> high e - i e) (dnfp_mon v) (\<lambda>x y. high y - i y \<le> high e - i e)"
-  apply(induction v rule: dnfp_mon.induct)
-    apply(simp add: spec_def)
-    apply (simp add: skip_def)
-  apply(simp only: caseN)
-  apply(intro get_rule; intro allI; clarify)
-  apply(intro cond_rule)
-  apply(simp add: loop_update_action_def)
-  apply(intro get_rule; intro allI; clarify)
-  apply(intro seq_rule[of _ _ "(\<lambda>x y. high y - i y \<le> high e - i e)"])
-  apply(intro cond_rule)
-  apply(simp add: inc_lowbound_def)
-   apply(intro get_rule; intro allI; simp)
-  apply(intro seq_rule[of _ _ "(\<lambda>x y. high y - i y \<le> high e - i e)"])
-    apply(simp add: spec_def put_def xs_Env_def swap_def put_state_def get_state_def)
-   apply(intro allI; simp)
-   apply(intro get_rule; intro allI)
-  apply(intro seq_rule[of _ _ "(\<lambda>x y. high y - i y \<le> high e - i e)"])
-   apply(simp add: spec_def put_def i_Env_def put_state_def get_state_def)
-  apply (simp add: le_diff_conv)
-   apply(intro allI; simp)
-   apply(intro get_rule; intro allI)
-    apply(simp add: spec_def put_def low_Env_def put_state_def get_state_def)
-  apply(simp add: dec_highbound_def)
-   apply(intro get_rule; intro allI; simp)
-  apply(intro seq_rule[of _ _ "(\<lambda>x y. high y - i y \<le> high e - i e)"])
-  apply(simp add: spec_def put_def high_Env_def put_state_def get_state_def)
-  apply linarith
-   apply(intro allI; simp)
-  apply(intro get_rule; intro allI; simp)
-    apply(simp add: spec_def put_def xs_Env_def swap_def put_state_def get_state_def)
-  apply(simp add: inc_index_def)
-  apply(intro get_rule; intro allI; simp)
-    apply(simp add: spec_def put_def i_Env_def put_state_def get_state_def)
-  apply (simp add: le_diff_conv)
-   apply blast
-  apply(simp add: spec_def)
-  by (simp add: skip_def)
-
-lemma dnfp_aux6: "spec (\<lambda>y. mset (xs e) = mset (xs y)) (dnfp_mon v) (\<lambda>x y. mset (xs e) = mset (xs y))"
-  apply(induction v rule: dnfp_mon.induct)
-    apply(simp add: spec_def)
-    apply (simp add: skip_def)
-  apply(simp only: caseN)
-  apply(intro get_rule; intro allI; clarify)
-  apply(intro cond_rule)
-  apply(simp add: loop_update_action_def)
-  apply(intro get_rule; intro allI; clarify)
-  apply(intro seq_rule[of _ _ "(\<lambda>x y. mset (xs e) = mset (xs y))"])
-  apply(intro cond_rule)
-  apply(simp add: inc_lowbound_def)
-  apply(intro get_rule; intro allI; simp)
-  apply(intro seq_rule[of _ _ "(\<lambda>x y. mset (xs e) = mset (xs y))"])
-  apply(simp add: spec_def put_def xs_Env_def swap_def put_state_def get_state_def)
-  apply (simp add: Multiset.mset_swap)
-  apply(intro allI; simp)
-  apply(intro get_rule; intro allI)
-  apply(intro seq_rule[of _ _ "(\<lambda>x y. mset (xs e) = mset (xs y))"])
-  apply(simp add: spec_def put_def i_Env_def put_state_def get_state_def)
-  apply(intro allI; simp)
-  apply(intro get_rule; intro allI)
-  apply(simp add: spec_def put_def low_Env_def put_state_def get_state_def)
-  apply(simp add: dec_highbound_def)
-  apply(intro get_rule; intro allI; simp)
-  apply(intro seq_rule[of _ _ "(\<lambda>x y. mset (xs e) = mset (xs y))"])
-  apply(simp add: spec_def put_def high_Env_def put_state_def get_state_def)
-  apply(intro allI; simp)
-  apply(intro get_rule; intro allI; simp)
-  apply(simp add: spec_def put_def xs_Env_def swap_def put_state_def get_state_def)
-  apply (simp add: Multiset.mset_swap)
-  apply(simp add: inc_index_def)
-  apply(intro get_rule; intro allI; simp)
-  apply(simp add: spec_def put_def i_Env_def put_state_def get_state_def)
-  apply blast
-  apply(simp add: spec_def)
-  by (simp add: skip_def)
-
-subsection\<open>DNFP proof\<close>
-lemma dnfp_prepost: "spec (dnfp_pre n e) (dnfp_mon n) (GG (dnfp_post e))"
-  apply(induction rule: dnfp_mon.induct)
-  unfolding dnfp_pre_def dnfp_pre_aux_def GG_def dnfp_post_def
-    apply(simp add: spec_def)
-   apply (simp add: skip_def)
-  apply(intro conj_rule_right; simp only: caseN)
-   apply(intro get_rule; intro allI; clarify)
-   apply(intro cond_rule; simp)
-  apply(simp add: loop_update_action_def)
-  apply(intro get_rule; intro allI; clarify)
-  apply(intro seq_rule[of _ _ "(\<lambda>x y. length (xs e) = length (xs y))"])
-  apply(intro cond_rule)
-  apply(simp add: inc_lowbound_def)
-   apply(intro get_rule; intro allI; simp)
-  apply(intro seq_rule[of _ _ "(\<lambda>x y. length (xs e) = length (xs y))"])
-    apply(simp add: spec_def put_def xs_Env_def swap_def put_state_def get_state_def)
-   apply(intro allI; simp)
-   apply(intro get_rule; intro allI)
-  apply(intro seq_rule[of _ _ "(\<lambda>x y. length (xs e) = length (xs y))"])
-    apply(simp add: spec_def put_def i_Env_def put_state_def get_state_def)
-   apply(intro allI; simp)
-         apply(intro get_rule; intro allI)
-    apply(simp add: spec_def put_def low_Env_def put_state_def get_state_def)
-  apply(simp add: dec_highbound_def)
-   apply(intro get_rule; intro allI; simp)
-  apply(intro seq_rule[of _ _ "(\<lambda>x y. length (xs e) = length (xs y))"])
-    apply(simp add: spec_def put_def high_Env_def put_state_def get_state_def)
-   apply(intro allI; simp)
-  apply(intro get_rule; intro allI; simp)
-    apply(simp add: spec_def put_def xs_Env_def swap_def put_state_def get_state_def)
-  apply(simp add: inc_index_def)
-  apply(intro get_rule; intro allI; simp)
-    apply(simp add: spec_def put_def i_Env_def put_state_def get_state_def)
-        apply(intro allI; simp)
-  using dnfp_aux1 apply blast
-        apply(simp add: spec_def skip_def)
-   apply(intro get_rule; intro allI; clarify)
-       apply(intro cond_rule)
-  apply(simp add: loop_update_action_def)
-  apply(intro get_rule; intro allI; clarify)
-  apply(intro seq_rule[of _ _ "(\<lambda>x y. high y \<le> high e)"])
-       apply(intro cond_rule)
- apply(simp add: inc_lowbound_def)
-   apply(intro get_rule; intro allI; simp)
-  apply(intro seq_rule[of _ _ "(\<lambda>x y. high y \<le> high e)"])
-    apply(simp add: spec_def put_def xs_Env_def swap_def put_state_def get_state_def)
-   apply(intro allI; simp)
-   apply(intro get_rule; intro allI)
-  apply(intro seq_rule[of _ _ "(\<lambda>x y. high y \<le> high e)"])
-    apply(simp add: spec_def put_def i_Env_def put_state_def get_state_def)
-   apply(intro allI; simp)
-         apply(intro get_rule; intro allI)
-    apply(simp add: spec_def put_def low_Env_def put_state_def get_state_def)
-  apply(simp add: dec_highbound_def)
-   apply(intro get_rule; intro allI; simp)
-  apply(intro seq_rule[of _ _ "(\<lambda>x y. high y \<le> high e)"])
-    apply(simp add: spec_def put_def high_Env_def put_state_def get_state_def)
-   apply(intro allI; simp)
-  apply(intro get_rule; intro allI; simp)
-    apply(simp add: spec_def put_def xs_Env_def swap_def put_state_def get_state_def)
-  apply(simp add: inc_index_def)
-  apply(intro get_rule; intro allI; simp)
-    apply(simp add: spec_def put_def i_Env_def put_state_def get_state_def)
-       apply(intro allI; simp)
-  using dnfp_aux2 apply blast
-    apply(simp add: spec_def skip_def)
-
-   apply(intro get_rule; intro allI; clarify)
-       apply(intro cond_rule)
-  apply(simp add: loop_update_action_def)
-  apply(intro get_rule; intro allI; clarify)
-  apply(intro seq_rule[of _ _ "(\<lambda>x y. low e \<le> low y)"])
-       apply(intro cond_rule)
- apply(simp add: inc_lowbound_def)
-   apply(intro get_rule; intro allI; simp)
-  apply(intro seq_rule[of _ _ "(\<lambda>x y. low e \<le> low y)"])
-    apply(simp add: spec_def put_def xs_Env_def swap_def put_state_def get_state_def)
-   apply(intro allI; simp)
-   apply(intro get_rule; intro allI)
-  apply(intro seq_rule[of _ _ "(\<lambda>x y. low e \<le> low y)"])
-    apply(simp add: spec_def put_def i_Env_def put_state_def get_state_def)
-   apply(intro allI; simp)
-         apply(intro get_rule; intro allI)
-    apply(simp add: spec_def put_def low_Env_def put_state_def get_state_def)
-  apply(simp add: dec_highbound_def)
-   apply(intro get_rule; intro allI; simp)
-  apply(intro seq_rule[of _ _ "(\<lambda>x y. low e \<le> low y)"])
-    apply(simp add: spec_def put_def high_Env_def put_state_def get_state_def)
-   apply(intro allI; simp)
-  apply(intro get_rule; intro allI; simp)
-    apply(simp add: spec_def put_def xs_Env_def swap_def put_state_def get_state_def)
-  apply(simp add: inc_index_def)
-  apply(intro get_rule; intro allI; simp)
-    apply(simp add: spec_def put_def i_Env_def put_state_def get_state_def)
-  using dnfp_aux3 apply blast
-  apply(simp add: spec_def skip_def)
-
-   apply(intro get_rule; intro allI; clarify)
-       apply(intro cond_rule)
-  apply(simp add: loop_update_action_def)
-  apply(intro get_rule; intro allI; clarify)
-  apply(intro seq_rule[of _ _ "(\<lambda>x y. i e \<le> i y)"])
-       apply(intro cond_rule)
- apply(simp add: inc_lowbound_def)
-   apply(intro get_rule; intro allI; simp)
-  apply(intro seq_rule[of _ _ "(\<lambda>x y. i e \<le> i y)"])
-    apply(simp add: spec_def put_def xs_Env_def swap_def put_state_def get_state_def)
-   apply(intro allI; simp)
-   apply(intro get_rule; intro allI)
-  apply(intro seq_rule[of _ _ "(\<lambda>x y. i e \<le> i y)"])
-    apply(simp add: spec_def put_def i_Env_def put_state_def get_state_def)
-   apply(intro allI; simp)
-         apply(intro get_rule; intro allI)
-    apply(simp add: spec_def put_def low_Env_def put_state_def get_state_def)
-  apply(simp add: dec_highbound_def)
-   apply(intro get_rule; intro allI; simp)
-  apply(intro seq_rule[of _ _ "(\<lambda>x y. i e \<le> i y)"])
-    apply(simp add: spec_def put_def high_Env_def put_state_def get_state_def)
-   apply(intro allI; simp)
-  apply(intro get_rule; intro allI; simp)
-    apply(simp add: spec_def put_def xs_Env_def swap_def put_state_def get_state_def)
-  apply(simp add: inc_index_def)
-  apply(intro get_rule; intro allI; simp)
-    apply(simp add: spec_def put_def i_Env_def put_state_def get_state_def)
-  using dnfp_aux4 apply blast
-  apply(simp add: spec_def skip_def)
-
-   apply(intro get_rule; intro allI; clarify)
-       apply(intro cond_rule)
-  apply(simp add: loop_update_action_def)
-  apply(intro get_rule; intro allI; clarify)
-  apply(intro seq_rule[of _ _ "(\<lambda>x y. high y - i y \<le> high e - i e)"])
-       apply(intro cond_rule)
- apply(simp add: inc_lowbound_def)
-   apply(intro get_rule; intro allI; simp)             
-  apply(intro seq_rule[of _ _ "(\<lambda>x y. high y - i y \<le> high e - i e)"])
-    apply(simp add: spec_def put_def xs_Env_def swap_def put_state_def get_state_def)
-   apply(intro allI; simp)
-   apply(intro get_rule; intro allI)
-  apply(intro seq_rule[of _ _ "(\<lambda>x y. high y - i y \<le> high e - i e)"])
-  apply(simp add: spec_def put_def i_Env_def put_state_def get_state_def)
-  apply (simp add: le_diff_conv)
-   apply(intro allI; simp)
-   apply(intro get_rule; intro allI)
-  apply(simp add: spec_def put_def low_Env_def put_state_def get_state_def)
-  apply(simp add: dec_highbound_def)
-   apply(intro get_rule; intro allI; simp)
-  apply(intro seq_rule[of _ _ "(\<lambda>x y. high y - i y \<le> high e - i e)"])
-       apply(simp add: spec_def put_def high_Env_def put_state_def get_state_def)
-  apply linarith
-   apply(intro allI; simp)
-  apply(intro get_rule; intro allI; simp)
-    apply(simp add: spec_def put_def xs_Env_def swap_def put_state_def get_state_def)
-  apply(simp add: inc_index_def)
-  apply(intro get_rule; intro allI; simp)
-         apply(simp add: spec_def put_def i_Env_def put_state_def get_state_def)
-  apply linarith
-    apply(intro allI; simp)
-  using dnfp_aux5 apply blast
-  apply(simp add: spec_def skip_def)
-
- apply(intro get_rule; intro allI; clarify)
- apply(intro cond_rule)
-  apply(simp add: loop_update_action_def)
-  apply(intro get_rule; intro allI; clarify)
-  apply(intro seq_rule[of _ _ "(\<lambda>x y. mset (xs e) = mset (xs y))"])
-       apply(intro cond_rule)
- apply(simp add: inc_lowbound_def)
-   apply(intro get_rule; intro allI; simp)
-  apply(intro seq_rule[of _ _ "(\<lambda>x y. mset (xs e) = mset (xs y))"])
-            apply(simp add: spec_def put_def xs_Env_def swap_def put_state_def get_state_def)
-  apply (simp add: Multiset.mset_swap)
-   apply(intro allI; simp)
-   apply(intro get_rule; intro allI)
-  apply(intro seq_rule[of _ _ "(\<lambda>x y. mset (xs e) = mset (xs y))"])
-  apply(simp add: spec_def put_def i_Env_def put_state_def get_state_def)
-   apply(intro allI; simp)
-         apply(intro get_rule; intro allI)
-    apply(simp add: spec_def put_def low_Env_def put_state_def get_state_def)
-  apply(simp add: dec_highbound_def)
-   apply(intro get_rule; intro allI; simp)
-  apply(intro seq_rule[of _ _ "(\<lambda>x y. mset (xs e) = mset (xs y))"])
-  apply(simp add: spec_def put_def high_Env_def put_state_def get_state_def)
-   apply(intro allI; simp)
-  apply(intro get_rule; intro allI; simp)
-  apply(simp add: spec_def put_def xs_Env_def swap_def put_state_def get_state_def)
-  apply (simp add: Multiset.mset_swap)
-  apply(simp add: inc_index_def)
-  apply(intro get_rule; intro allI; simp)
-   apply(simp add: spec_def put_def i_Env_def put_state_def get_state_def)
-    apply(intro allI; simp)
-  using dnfp_aux6 apply blast
-  by(simp add: spec_def skip_def)
-
-subsection\<open>Invariants proof\<close>
+section\<open>DNFP proof\<close>
+subsection\<open>DNFP preserves the Invariants proof\<close>
 lemma dnfp_invariantRed: "spec (dnfp_inv1) (dnfp_mon n) (GG dnfp_inv1)"
   unfolding dnfp_inv1_def dnfp_pre_aux_def GG_def 
   apply(induction n rule: dnfp_mon.induct)
@@ -494,104 +77,18 @@ lemma dnfp_invariantBlue: "spec dnfp_inv3 (dnfp_mon n) (GG dnfp_inv3)"
      apply(simp add: spec_def)
   by(simp add: skip_def)
 
-section\<open>Main proof\<close>
-definition dnfp_mon_inv :: "env \<Rightarrow> bool" where
-"dnfp_mon_inv e \<equiv> ((dnfp_inv3 e) \<and> (dnfp_inv2 e) \<and> (dnfp_inv1 e))"
-
+text\<open>All invariants are preserved\<close>
 lemma dnfp_mon_invariants: "spec (dnfp_mon_inv) (dnfp_mon n) (GG dnfp_mon_inv)"
   by (smt GG_def dnfp_invariantBlue dnfp_invariantRed dnfp_invariantWhite dnfp_mon_inv_def invariants_Env_def spec_def split_def)
 
-definition dnfp_post_spec where
-"dnfp_post_spec e \<equiv> dnfp_mon_inv e \<and> i e = high e"
+section\<open>Main proof\<close>
 
-lemma dnfp_mon_isSorted: "dnfp_post_spec e \<Longrightarrow> sorted (xs e)" 
-  unfolding  dnfp_post_spec_def dnfp_mon_inv_def
+text\<open>If the invariants are kept and i = high, when the entire array will be sorted\<close>
+lemma dnfp_mon_isSorted: "dnfp_post_final_spec e \<Longrightarrow> sorted (xs e)" 
+  unfolding dnfp_post_final_spec_def dnfp_mon_inv_def
   by (smt Suc_1 Suc_leD dnfp_inv1_def dnfp_inv2_def dnfp_inv3_def high_invariant_is_2_Env_def invariant_low_to_j_is_1_Env_def less_numeral_extra(1) less_or_eq_imp_le less_trans low_invariant_is_0_Env_def not_less sorted_iff_nth_mono_less)
 
-definition dnfp_post_spec1 where
-"dnfp_post_spec1 e \<equiv> dnfp_mon_inv e \<and> i e = high e \<and> sorted(xs e)"
-
-definition range_0:: "env \<Rightarrow> nat array" where
-"range_0 e \<equiv> nths (xs e) (set(upt 0 (low e)))"
-
-definition range_1:: "env \<Rightarrow> nat array" where
-"range_1 e \<equiv> nths (xs e) (set(upt (low e) (i e)))"
-
-definition range_2:: "env \<Rightarrow> nat array" where
-"range_2 e \<equiv> nths (xs e) (set(upt (high e) (length (xs e))))"
-
-lemma as: "nths x {0..<z} = take z x"
-  by (simp add: atLeast0LessThan)
-
-(*I don't get why I can't prove this*)
-lemma as1: "\<lbrakk>n = length x; z < n\<rbrakk> \<Longrightarrow> nths x {0..<z} @ nths x {z..<n}= take n x"
-  apply(induction n arbitrary: x)
-   apply simp
-  sorry
-
-lemma complete_range_aux: "\<lbrakk>n = length x; z < length x\<rbrakk> \<Longrightarrow> nths x {0..<z} @ nths x {z..<n} = x"
-  apply(induction n arbitrary: z)
-   apply simp
-  by (simp add: as1)
-
-
-lemma complete_range: "\<lbrakk>z \<le> y; n = length x; y < length x\<rbrakk> \<Longrightarrow> nths x {0..<z} @ nths x {z..<y} @ nths x {y..<n} = x"
-  apply(induction n arbitrary: z y x)
-   apply simp
-  sorry
-
-lemma range_isComplete: "\<lbrakk>dnfp_precondition e; high e = i e\<rbrakk> \<Longrightarrow> concat[range_0 e, range_1 e,  range_2 e] = xs e"
-  unfolding range_0_def range_1_def range_2_def dnfp_precondition_def
-  apply(auto)
-  by (metis append.simps(1) append_Nil2 atLeastLessThan0 atLeastLessThan_empty_iff complete_range le0 le_SucE le_neq_implies_less le_numeral_extra(3) le_zero_eq length_0_conv less_Suc_eq_0_disj nths_empty same_append_eq set_upt zero_induct)
-
-definition sorted_range_get:: "env \<Rightarrow> nat array" where
-"sorted_range_get e \<equiv> range_0 e @ range_1 e @ range_2 e"
-
-definition sorted_range:: "env \<Rightarrow> bool" where
-"sorted_range e \<equiv> sorted(sorted_range_get e)"
-
-lemma range_0_isZero: "low_invariant_is_0_Env e \<Longrightarrow> \<forall>x \<in> set(range_0 e). x = 0"
-  unfolding low_invariant_is_0_Env_def range_0_def
-  by (smt atLeast_upt lessThan_iff mem_Collect_eq set_nths)
-
-lemma range_0_sorted: "dnfp_mon_inv e \<Longrightarrow> sorted (range_0 e)"
-  unfolding dnfp_mon_inv_def dnfp_inv3_def dnfp_inv2_def dnfp_inv1_def range_1_def dnfp_precondition_def
-  by (metis eq_iff less_trans nth_mem range_0_isZero sorted_iff_nth_mono_less)
-
-lemma range_1_isOne: "invariant_low_to_j_is_1_Env e \<Longrightarrow> \<forall>x \<in> set(range_1 e). x = 1"
-  unfolding invariant_low_to_j_is_1_Env_def range_1_def
-  by (smt atLeastLessThan_iff mem_Collect_eq set_nths set_upt)
-
-lemma range_1_sorted: "dnfp_mon_inv e \<Longrightarrow> sorted (range_1 e)"
-  by (smt diff_is_0_eq dnfp_inv2_def dnfp_mon_inv_def le_neq_implies_less length_take less_trans min.absorb2 nat_le_linear not_one_less_zero nth_mem range_1_def range_1_isOne sorted01 sorted_iff_nth_mono take_all)
-
-lemma ranges_sorted: "\<lbrakk>invariant_low_to_j_is_1_Env e; low_invariant_is_0_Env e\<rbrakk> \<Longrightarrow> sorted(range_0 e @ range_1 e)"
-  by (metis less_trans nat_le_linear not_one_le_zero nth_mem range_0_isZero range_1_isOne sorted_append sorted_iff_nth_mono_less)
-
-lemma range_2_isTwo: "high_invariant_is_2_Env e \<Longrightarrow> \<forall>x \<in> set(range_2 e). x = 2"
-  unfolding high_invariant_is_2_Env_def range_2_def
-  by (smt atLeastLessThan_iff mem_Collect_eq set_nths set_upt)
-
-lemma range_2_sorted: "dnfp_mon_inv e \<Longrightarrow> sorted (range_2 e)"
-  by (metis dnfp_inv3_def dnfp_mon_inv_def eq_iff less_trans nth_mem range_2_isTwo sorted_sorted_wrt sorted_wrt_iff_nth_less)
-
-lemma "dnfp_mon_inv e \<Longrightarrow> sorted(sorted_range_get e)"
-  by (metis Suc_1 dnfp_inv1_def dnfp_inv2_def dnfp_inv3_def dnfp_mon_inv_def lessI less_imp_le_nat range_0_isZero range_0_sorted range_1_isOne range_1_sorted range_2_isTwo range_2_sorted sorted_append sorted_range_get_def zero_le)
-
-lemma sorted_aux: "dnfp_mon_inv e \<Longrightarrow> sorted_range e"
-  unfolding sorted_range_def
-  by (metis Suc_1 dnfp_inv1_def dnfp_inv2_def dnfp_inv3_def dnfp_mon_inv_def lessI less_imp_le_nat range_0_isZero range_0_sorted range_1_isOne range_1_sorted range_2_isTwo range_2_sorted sorted_append sorted_range_get_def zero_le)
-
-lemma "sorted_range e \<and> i e = high e \<and> dnfp_precondition e \<Longrightarrow> sorted (xs e)"
-  unfolding sorted_range_def sorted_range_get_def dnfp_precondition_def
-  using dnfp_precondition_def range_isComplete by auto
-
-definition dnfp_mon_spec where
-"dnfp_mon_spec e \<equiv> dnfp_precondition e
-                    \<and> dnfp_mon_inv e
-                    \<and> sorted_range e"
-
+text\<open>DNFP mon preserves the invariants on the ranges and the bounds of the variables\<close>
 lemma dnfp_mon_main: "spec (dnfp_mon_spec) (dnfp_mon n) (GG dnfp_mon_spec)"
   unfolding GG_def dnfp_mon_spec_def
   apply(induction n rule: dnfp_mon.induct)
@@ -602,37 +99,13 @@ lemma dnfp_mon_main: "spec (dnfp_mon_spec) (dnfp_mon n) (GG dnfp_mon_spec)"
   apply(intro cond_rule)
    apply(simp add: loop_update_action_def)
    apply(intro get_rule; intro allI; clarify)
-   apply(intro seq_rule[of _ _ "(\<lambda>x e. dnfp_precondition e \<and> dnfp_mon_inv e \<and> sorted_range e)"])
+   apply(intro seq_rule[of _ _ "(\<lambda>x e. dnfp_precondition e \<and> dnfp_mon_inv e)"])
     apply(intro cond_rule)
-      apply(intro conj_rule_right; simp)
-  apply (smt GG_def dnfp_inv1_def dnfp_mon_inv_def inc_lowbound_inv1_aux_def inc_lowbound_inv1_def inc_lowbound_invariantRed less_numeral_extra(1) loop_update_action_pre_def spec_def split_beta')
-  apply (smt GG_def Pair_inject dnfp_inv1_def dnfp_inv2_def dnfp_inv3_def dnfp_mon_inv_def inc_lowbound_inv1_aux_def inc_lowbound_inv1_def inc_lowbound_inv2_aux_def inc_lowbound_inv2_def inc_lowbound_inv3_aux_def inc_lowbound_inv3_def inc_lowbound_invariantBlue inc_lowbound_invariantRed inc_lowbound_invariantWhite less_one loop_update_action_pre_def spec_def split_beta')
-  apply (smt Dutch_National_Flag_Monad.sorted_aux GG_def dnfp_inv1_def dnfp_inv2_def dnfp_inv3_def dnfp_mon_inv_def inc_lowbound_inv1_aux_def inc_lowbound_inv1_def inc_lowbound_inv2_aux_def inc_lowbound_inv2_def inc_lowbound_inv3_aux_def inc_lowbound_inv3_def inc_lowbound_invariantBlue inc_lowbound_invariantRed inc_lowbound_invariantWhite less_numeral_extra(1) loop_update_action_pre_def spec_def split_beta')
-      apply(intro conj_rule_right)
-        apply (smt GG_def Pair_inject dec_highbound_inv1_aux_def dec_highbound_inv1_def dec_highbound_invariantRed dnfp_inv1_def dnfp_mon_inv_def loop_update_action_pre_def spec_def split_beta')
-      apply (smt GG_def Pair_inject dec_highbound_inv1_aux_def dec_highbound_inv1_def dec_highbound_inv2_aux_def dec_highbound_inv2_def dec_highbound_inv3_aux_def dec_highbound_inv3_def dec_highbound_invariantBlue dec_highbound_invariantRed dec_highbound_invariantWhite dnfp_inv1_def dnfp_inv2_def dnfp_inv3_def dnfp_mon_inv_def loop_update_action_pre_def spec_def split_beta')
-      apply (smt Dutch_National_Flag_Monad.sorted_aux GG_def Pair_inject dec_highbound_inv1_aux_def dec_highbound_inv1_def dec_highbound_inv2_aux_def dec_highbound_inv2_def dec_highbound_inv3_aux_def dec_highbound_inv3_def dec_highbound_invariantBlue dec_highbound_invariantRed dec_highbound_invariantWhite dnfp_inv1_def dnfp_inv2_def dnfp_inv3_def dnfp_mon_inv_def loop_update_action_pre_def spec_def split_beta')
-      apply(intro conj_rule_right)
-        apply (smt GG_def Pair_inject dnfp_inv1_def dnfp_mon_inv_def inc_index_inv1_aux_def inc_index_inv1_def inc_index_invariantRed less_one loop_update_action_pre_def spec_def split_beta')
-     apply (smt GG_def Pair_inject dnfp_inv1_def dnfp_inv2_def dnfp_inv3_def dnfp_mon_inv_def inc_index_inv1_aux_def inc_index_inv1_def inc_index_inv2_aux_def inc_index_inv2_def inc_index_inv3_aux_def inc_index_inv3_def inc_index_invariantBlue inc_index_invariantRed inc_index_invariantWhite less_one loop_update_action_pre_def spec_def split_beta')
-  apply (smt Dutch_National_Flag_Monad.sorted_aux GG_def Pair_inject dnfp_inv1_def dnfp_inv2_def dnfp_inv3_def dnfp_mon_inv_def inc_index_inv1_aux_def inc_index_inv1_def inc_index_inv2_aux_def inc_index_inv2_def inc_index_inv3_aux_def inc_index_inv3_def inc_index_invariantBlue inc_index_invariantRed inc_index_invariantWhite less_one loop_update_action_pre_def spec_def split_beta')
+      apply (smt GG_def Pair_inject dnfp_inv1_def dnfp_inv2_def dnfp_inv3_def dnfp_mon_inv_def inc_lowbound_inv1_aux_def inc_lowbound_inv1_def inc_lowbound_inv2_aux_def inc_lowbound_inv2_def inc_lowbound_inv3_aux_def inc_lowbound_inv3_def inc_lowbound_invariantBlue inc_lowbound_invariantRed inc_lowbound_invariantWhite less_numeral_extra(1) loop_update_action_pre_def spec_def split_beta')
+  apply (smt GG_def Pair_inject dec_highbound_inv1_aux_def dec_highbound_inv1_def dec_highbound_inv2_aux_def dec_highbound_inv2_def dec_highbound_inv3_aux_def dec_highbound_inv3_def dec_highbound_invariantBlue dec_highbound_invariantRed dec_highbound_invariantWhite dnfp_inv1_def dnfp_inv2_def dnfp_inv3_def dnfp_mon_inv_def loop_update_action_pre_def spec_def split_beta')
+  apply (smt GG_def Pair_inject dnfp_inv1_def dnfp_inv2_def dnfp_inv3_def dnfp_mon_inv_def inc_index_inv1_aux_def inc_index_inv1_def inc_index_inv2_aux_def inc_index_inv2_def inc_index_inv3_aux_def inc_index_inv3_def inc_index_invariantBlue inc_index_invariantRed inc_index_invariantWhite less_one loop_update_action_pre_def spec_def split_beta') 
   apply blast
   by(simp add: spec_def skip_def)
-
-(*
-  add precondition:
-  Everything outside n is sorted
-  high to n
-  And finally everything should be sorted
-  Post condition high = i 
-*)
-
-
-definition i_high_equal::"nat \<Rightarrow> env \<Rightarrow> bool"  where
- "i_high_equal n e \<equiv> high e = i e"
-
-definition dnfp_mon_pre::"nat \<Rightarrow> env \<Rightarrow> bool"  where
-"dnfp_mon_pre n e \<equiv> dnfp_precondition e \<and> n = high e - i e"
 
 lemma aux1: "(spec (\<lambda>e. dnfp_precondition e \<and> n = high e - i e) (dnfp_mon n)
                 (\<lambda>x e. high e = i e)) \<Longrightarrow>
@@ -672,7 +145,16 @@ lemma aux1: "(spec (\<lambda>e. dnfp_precondition e \<and> n = high e - i e) (dn
   apply linarith
   by blast
 
-lemma dnfp_mon_main_aux: "spec (dnfp_mon_pre n) (dnfp_mon n) (GG (i_high_equal n))"
+subsection\<open>Main proofs\<close>
+definition dnfp_mon_pre::"nat \<Rightarrow> env \<Rightarrow> bool"  where
+"dnfp_mon_pre n e \<equiv> dnfp_precondition e \<and> n = high e - i e"
+
+definition i_high_equal::"nat \<Rightarrow> env \<Rightarrow> bool"  where
+ "i_high_equal n e \<equiv> high e = i e"
+
+text\<open>If dnfp is called with a proper environment and n is the difference between high and i. When High and I will be equal after the termination of the function.
+This can be used the termination. And this proof can together with the dnfp_mon_main-proof be used to proof that the array will be sorted by the dnfp-function\<close>
+lemma dnfp_mon_termination: "spec (dnfp_mon_pre n) (dnfp_mon n) (GG (i_high_equal n))"
   unfolding GG_def dnfp_mon_pre_def dnfp_mon_spec_def i_high_equal_def
   apply(induction n rule: dnfp_mon.induct)
     apply(simp add: spec_def)
@@ -687,15 +169,26 @@ lemma dnfp_mon_main_aux: "spec (dnfp_mon_pre n) (dnfp_mon n) (GG (i_high_equal n
 definition dnfp_mon_spec_aux:: "nat \<Rightarrow> env \<Rightarrow> bool" where
 "dnfp_mon_spec_aux n e \<equiv> n = high e - i e \<and> dnfp_mon_spec e"
 
-definition list_sorted where
-"list_sorted e \<equiv> sorted(xs e)"
+definition array_sorted where
+"array_sorted e \<equiv> sorted(xs e)"
 
-lemma dnfp_mon_main_list_sorted: "spec (dnfp_mon_spec_aux n) (dnfp_mon n) (GG list_sorted)"
-  unfolding GG_def dnfp_mon_spec_aux_def  list_sorted_def
+lemma dnfp_mon_main_list_sorted: "spec (dnfp_mon_spec_aux n) (dnfp_mon n) (GG array_sorted)"
+  unfolding GG_def dnfp_mon_spec_aux_def array_sorted_def
   apply(induction n rule: dnfp_mon.induct)
-    apply(simp add: spec_def)
-   apply(simp add: skip_def)
-  apply (simp add: dnfp_mon_isSorted dnfp_mon_spec_def dnfp_post_spec_def dnfp_precondition_def)
-  by (smt GG_def dnfp_mon_invariants dnfp_mon_isSorted dnfp_mon_main_aux dnfp_mon_pre_def dnfp_mon_spec_def dnfp_post_spec_def i_high_equal_def spec_def split_beta')
+  apply (simp add: spec_def skip_def dnfp_mon_isSorted dnfp_mon_spec_def dnfp_post_final_spec_def dnfp_precondition_def)
+  by (smt GG_def dnfp_mon_invariants dnfp_mon_isSorted dnfp_mon_termination dnfp_mon_pre_def dnfp_mon_spec_def dnfp_post_final_spec_def i_high_equal_def spec_def split_beta')
+
+section\<open>Examples of DNFP\<close>
+definition init_env:: "nat array \<Rightarrow> env" where
+  "init_env l \<equiv> \<lparr>high = (length l),            low = 0,
+                 i = 0,                         xs = l\<rparr>"
+
+value \<open>snd(run_state (dnfp_mon 5) (init_env [0,2,2,1,2]))\<close>
+value \<open>snd(run_state (dnfp_mon 9) (init_env [0,2,2,0,1,0,2,1,2]))\<close>
+value \<open>snd(run_state (dnfp_mon 3)(init_env [2,1,0]))\<close>
+
+value \<open>assert(sorted(xs(snd(run_state (dnfp_mon 5) (init_env[0,2,2,1,2])))))\<close>
+value \<open>assert(sorted(xs(snd(run_state (dnfp_mon 9) (init_env[0,2,2,0,1,0,2,1,2])))))\<close>
+value \<open>assert(sorted(xs(snd(run_state (dnfp_mon 3) (init_env[2,1,0])))))\<close>
 
 end
