Monad_Play Around/DNFP/Dutch_National_Flag_Monad_Definitions.thy
@@ -13,7 +13,7 @@ record env =
   i    :: "nat"
   xs   :: "nat array"
 
-subsection\<open>update functions\<close>
+subsection\<open>Monad update functions\<close>
 definition high_Env:: "env \<Rightarrow> nat \<Rightarrow> env" where "high_Env s v = s \<lparr> high := v \<rparr>"
 definition low_Env:: "env \<Rightarrow> nat \<Rightarrow> env" where "low_Env s v = s \<lparr> low := v \<rparr>"
 definition i_Env:: "env \<Rightarrow> nat \<Rightarrow> env" where "i_Env s v = s \<lparr> i := v \<rparr>"
@@ -86,24 +86,8 @@ definition loop_update_action where
   }"
 
 
-definition init_env:: "nat array \<Rightarrow> env" where
-  "init_env l \<equiv> \<lparr>high = (length l),            low = 0,
-                 i = 0,                         xs = l\<rparr>"
-
-definition init_state_env:: "nat array \<Rightarrow> (env, unit) state" where
-  "init_state_env l \<equiv> State (\<lambda>x. ((),init_env l))"
-
-value \<open>snd(run_state (dnfp_mon 5) (init_env [0,2,2,1,2]))\<close>
-value \<open>snd(run_state (dnfp_mon 9) (init_env [0,2,2,0,1,0,2,1,2]))\<close>
-value \<open>snd(run_state (dnfp_mon 3)(init_env [2,1,0]))\<close>
-
-value \<open>sorted(xs(snd(run_state (dnfp_mon 5) (init_env[0,2,2,1,2]))))\<close>
-value \<open>sorted(xs(snd(run_state (dnfp_mon 9) (init_env[0,2,2,0,1,0,2,1,2]))))\<close>
-value \<open>sorted(xs(snd(run_state (dnfp_mon 3) (init_env[2,1,0]))))\<close>
-
-section\<open>Definiton of all the Pre and postconditions\<close>
-
-subsection\<open>The invariants are taken from https://en.wikipedia.org/wiki/Dutch_national_flag_problem\<close>
+section\<open>Invariants definitions\<close>
+text\<open>The invariants are taken from https://en.wikipedia.org/wiki/Dutch_national_flag_problem\<close>
 definition low_invariant_is_0_Env where
 "low_invariant_is_0_Env e \<equiv> (\<forall>x. x < (low e) \<longrightarrow> (xs e)!x = 0)"
 
@@ -118,26 +102,24 @@ definition invariants_Env:: "env \<Rightarrow> bool" where
               \<and> invariant_low_to_j_is_1_Env e
               \<and> low_invariant_is_0_Env e"
 
-text\<open>This can be used in the other pre and post-conditions for the methods inside loop_update_actions\<close>
-
-subsection\<open>Pre- and Postconditions\<close>
-
-subsubsection\<open>Pre-conditions\<close>
+section\<open>General DNFP conditions\<close>
 definition dnfp_precondition:: "env \<Rightarrow> bool" where
 "dnfp_precondition e \<equiv> high e \<ge> i e
                       \<and> i e \<ge> low e 
                       \<and> length (xs e) \<ge> high e
                       \<and> set (xs e) \<subseteq> {0,1,2}"
 
-definition dnfp_pre_aux:: "nat \<Rightarrow> env \<Rightarrow> bool" where
-"dnfp_pre_aux n e \<equiv> 
-              dnfp_precondition e
-              \<and> high e - i e = n"
+definition dnfp_post where 
+"dnfp_post e e2 \<equiv> length (xs e) = length (xs e2)
+                  \<and> high e \<ge> high e2
+                  \<and> low e \<le> low e2
+                  \<and> i e \<le> i e2
+                  \<and> high e - i e \<ge> high e2 - i e2
+                  \<and> mset (xs e) = mset (xs e2)"
 
-definition dnfp_pre:: "nat \<Rightarrow> env \<Rightarrow> env \<Rightarrow> bool" where
-"dnfp_pre n e s \<equiv> s = e
-              \<and> dnfp_pre_aux n e"
-
+subsection\<open>Loop update action definitions\<close>
+text\<open>These definitions rely on the definitions on dnfp, but in the precondition they have an extra assumption that gets inferred from the conditions-statement inside the function\<close>
+text\<open>The post-condition is also for each of the definitions a little stronger compared to the more general\<close>
 
 definition loop_update_action_pre:: "env \<Rightarrow> bool" where
 "loop_update_action_pre e \<equiv> dnfp_precondition e \<and> high e > i e"
@@ -145,6 +127,12 @@ definition loop_update_action_pre:: "env \<Rightarrow> bool" where
 definition loop_update_action_pre_aux:: "env \<Rightarrow> env \<Rightarrow> bool" where
 "loop_update_action_pre_aux e s \<equiv> s = e
                               \<and> loop_update_action_pre e"
+
+definition loop_update_action_post where
+"loop_update_action_post e e' \<equiv> dnfp_post e e'
+                                \<and> high e - i e = Suc(high e' - i e')"
+
+subsubsection\<open>Loop update action Invariants\<close>
 
 definition loop_update_action_inv1 where 
 "loop_update_action_inv1 e \<equiv> dnfp_precondition e 
@@ -158,77 +146,73 @@ definition loop_update_action_inv3 where
 "loop_update_action_inv3 e \<equiv> dnfp_precondition e 
                               \<and> high_invariant_is_2_Env e"
 
-definition dnfp_post where 
-"dnfp_post e e2 \<equiv> length (xs e) = length (xs e2)
-                  \<and> high e \<ge> high e2
-                  \<and> low e \<le> low e2
-                  \<and> i e \<le> i e2
-                  \<and> high e - i e \<ge> high e2 - i e2
-                  \<and> mset (xs e) = mset (xs e2)"
-(*This needs to change a little bit*)
+definition loop_update_action_inv1_aux:: "env \<Rightarrow> bool" where
+"loop_update_action_inv1_aux e \<equiv> loop_update_action_inv1 e \<and> loop_update_action_pre e"
 
-definition loop_update_action_post where
-"loop_update_action_post e e' \<equiv> dnfp_post e e'
-                                \<and> high e - i e = Suc(high e' - i e')"
+definition loop_update_action_inv2_aux:: "env \<Rightarrow> bool" where
+"loop_update_action_inv2_aux e \<equiv> loop_update_action_inv2 e \<and> loop_update_action_pre e"
+
+definition loop_update_action_inv3_aux:: "env \<Rightarrow> bool" where
+"loop_update_action_inv3_aux e \<equiv> loop_update_action_inv3 e \<and> loop_update_action_pre e"     
+
+definition loop_update_action_inv :: "env \<Rightarrow> bool" where
+"loop_update_action_inv s \<equiv> (loop_update_action_inv3 s \<and> loop_update_action_inv2 s \<and> loop_update_action_inv1 s)"
+
+definition loop_update_action_inv_aux :: "env \<Rightarrow> bool" where
+"loop_update_action_inv_aux s \<equiv> (loop_update_action_inv s \<and> loop_update_action_pre s)"
+
+section\<open> Definitions of methods/definitions inside Loop_update action\<close>
+text\<open>These definitions rely on the definitions on loop_update_action, but in the precondition they have an extra assumption that gets inferred from the conditions-statement inside loop_update_action\<close>
+text\<open>The post-condition is also for each of the definitions a little stronger compared to the more general loop_update_action_post\<close>
+
+subsection\<open>Inc Lowbound definitions\<close>
 
 definition inc_lowbound_pre:: "env \<Rightarrow> env \<Rightarrow> bool" where 
 "inc_lowbound_pre e s \<equiv> s = e
                         \<and> loop_update_action_pre s
                         \<and> (xs s)!(i s) < 1"
 
-definition inc_lowbound_inv1 :: "env \<Rightarrow> bool" where
-"inc_lowbound_inv1 s \<equiv> dnfp_precondition s
-                        \<and> low_invariant_is_0_Env s"
-
-definition inc_lowbound_inv2 :: "env \<Rightarrow> bool" where
-"inc_lowbound_inv2 s \<equiv> dnfp_precondition s
-                        \<and> invariant_low_to_j_is_1_Env s"
-
-definition inc_lowbound_inv3 :: "env \<Rightarrow> bool" where
-"inc_lowbound_inv3 s \<equiv> dnfp_precondition s
-                        \<and> high_invariant_is_2_Env s"
-
-definition dec_highbound_pre where 
-"dec_highbound_pre e s\<equiv> e = s
-                        \<and> loop_update_action_pre e 
-                        \<and> (xs e)!(i e) > 1"
-
-definition dec_highbound_inv1 where 
-"dec_highbound_inv1 e \<equiv> dnfp_precondition e 
-                        \<and> low_invariant_is_0_Env e"
-
-definition dec_highbound_inv2 where 
-"dec_highbound_inv2 e \<equiv> dnfp_precondition e 
-                        \<and> invariant_low_to_j_is_1_Env e"
-
-definition dec_highbound_inv3 where 
-"dec_highbound_inv3 e \<equiv> dnfp_precondition e 
-                        \<and> high_invariant_is_2_Env e"
-
-definition inc_index_pre:: "env \<Rightarrow> env \<Rightarrow> bool" where 
-"inc_index_pre e s \<equiv> e = s 
-                      \<and> loop_update_action_pre e
-                      \<and> \<not>(xs e)!(i e) > 1
-                      \<and> \<not>(xs e)!(i e) < 1"
-
-definition inc_index_inv1:: "env \<Rightarrow> bool" where 
-"inc_index_inv1 e \<equiv> dnfp_precondition e
-                      \<and> low_invariant_is_0_Env e"
-
-definition inc_index_inv2:: "env \<Rightarrow> bool" where 
-"inc_index_inv2 e \<equiv> dnfp_precondition e
-                      \<and> invariant_low_to_j_is_1_Env e"
-
-definition inc_index_inv3:: "env \<Rightarrow> bool" where
-"inc_index_inv3 e \<equiv> dnfp_precondition e
-                    \<and> high_invariant_is_2_Env e"
-
-subsubsection\<open>Post-conditions\<close>
 definition inc_lowbound_post:: "env \<Rightarrow> env \<Rightarrow> bool" where 
 "inc_lowbound_post e e'\<equiv> high e = high e'
                           \<and> low e < low e'
                           \<and> loop_update_action_post e e'
                           \<and> i e < i e'"
+
+subsubsection\<open>Inc Index invariants\<close>
+
+definition inc_lowbound_inv1 :: "env \<Rightarrow> bool" where
+"inc_lowbound_inv1 s \<equiv> dnfp_precondition s
+                        \<and> low_invariant_is_0_Env s"
+
+definition inc_lowbound_inv1_aux:: "env \<Rightarrow> bool" where
+"inc_lowbound_inv1_aux e \<equiv> inc_lowbound_inv1 e \<and> loop_update_action_pre e \<and> xs e ! i e < 1"
+
+definition inc_lowbound_inv2 :: "env \<Rightarrow> bool" where
+"inc_lowbound_inv2 s \<equiv> dnfp_precondition s
+                        \<and> invariant_low_to_j_is_1_Env s"
+
+definition inc_lowbound_inv2_aux:: "env \<Rightarrow> bool" where
+"inc_lowbound_inv2_aux e \<equiv> inc_lowbound_inv2 e \<and> loop_update_action_pre e \<and> xs e ! i e < 1"
+
+definition inc_lowbound_inv3 :: "env \<Rightarrow> bool" where
+"inc_lowbound_inv3 s \<equiv> dnfp_precondition s
+                        \<and> high_invariant_is_2_Env s"
+
+definition inc_lowbound_inv3_aux:: "env \<Rightarrow> bool" where
+"inc_lowbound_inv3_aux e \<equiv> inc_lowbound_inv3 e \<and> loop_update_action_pre e \<and> xs e ! i e < 1"
+
+definition inc_lowbound_inv :: "env \<Rightarrow> bool" where
+"inc_lowbound_inv s \<equiv> (inc_lowbound_inv3 s \<and> inc_lowbound_inv2 s \<and> inc_lowbound_inv1 s)"
+
+definition inc_lowbound_inv_pre :: "env \<Rightarrow> bool" where
+"inc_lowbound_inv_pre s \<equiv> (inc_lowbound_inv s \<and> loop_update_action_pre s \<and> xs s ! i s < 1)"
+
+
+subsection\<open>Dec Highbound definitions\<close>
+definition dec_highbound_pre where 
+"dec_highbound_pre e s\<equiv> e = s
+                        \<and> loop_update_action_pre e 
+                        \<and> (xs e)!(i e) > 1"
 
 definition dec_highbound_post where 
 "dec_highbound_post e e' \<equiv> length (xs e') > high e' 
@@ -238,11 +222,78 @@ definition dec_highbound_post where
                               \<and> (xs e')!(high e') = 2
                               \<and> loop_update_action_post e e'"
 
+subsubsection\<open>Dec Highbound invariants\<close>
+definition dec_highbound_inv1 where 
+"dec_highbound_inv1 e \<equiv> dnfp_precondition e 
+                        \<and> low_invariant_is_0_Env e"
+
+definition dec_highbound_inv1_aux:: "env \<Rightarrow> bool" where
+"dec_highbound_inv1_aux e \<equiv> dec_highbound_inv1 e \<and> loop_update_action_pre e \<and> xs e ! i e > 1"
+
+definition dec_highbound_inv2 where 
+"dec_highbound_inv2 e \<equiv> dnfp_precondition e 
+                        \<and> invariant_low_to_j_is_1_Env e"
+
+definition dec_highbound_inv2_aux:: "env \<Rightarrow> bool" where
+"dec_highbound_inv2_aux e \<equiv> dec_highbound_inv2 e \<and> loop_update_action_pre e \<and> xs e ! i e > 1"
+
+definition dec_highbound_inv3 where 
+"dec_highbound_inv3 e \<equiv> dnfp_precondition e 
+                        \<and> high_invariant_is_2_Env e"
+
+definition dec_highbound_inv3_aux:: "env \<Rightarrow> bool" where
+"dec_highbound_inv3_aux e \<equiv> dec_highbound_inv3 e \<and> loop_update_action_pre e \<and> xs e ! i e > 1"
+
+
+definition dec_highbound_inv :: "env \<Rightarrow> bool" where
+"dec_highbound_inv s \<equiv> (dec_highbound_inv3 s \<and> dec_highbound_inv2 s \<and> dec_highbound_inv1 s)"
+
+definition dec_highbound_inv_aux :: "env \<Rightarrow> bool" where
+"dec_highbound_inv_aux s \<equiv> (dec_highbound_inv s \<and>  loop_update_action_pre s \<and> xs s ! i s > 1 )"
+
+
+subsection\<open>Inc index definitions\<close>
+definition inc_index_pre:: "env \<Rightarrow> env \<Rightarrow> bool" where 
+"inc_index_pre e s \<equiv> e = s 
+                      \<and> loop_update_action_pre e
+                      \<and> \<not>(xs e)!(i e) > 1
+                      \<and> \<not>(xs e)!(i e) < 1"
+
 definition inc_index_post:: "env \<Rightarrow> env \<Rightarrow> bool" where 
 "inc_index_post e e' \<equiv> high e = high e' 
                       \<and> low e = low e'
                       \<and> i e < i e'
                       \<and> loop_update_action_post e e'"
+
+subsubsection\<open>Inc index invariants\<close>
+definition inc_index_inv1:: "env \<Rightarrow> bool" where 
+"inc_index_inv1 e \<equiv> dnfp_precondition e
+                      \<and> low_invariant_is_0_Env e"
+
+definition inc_index_inv1_aux:: "env \<Rightarrow> bool" where
+"inc_index_inv1_aux e \<equiv> inc_index_inv1 e \<and> \<not>(xs e)!(i e) > 1 \<and> \<not>(xs e)!(i e) < 1 \<and> loop_update_action_pre e"
+
+definition inc_index_inv2:: "env \<Rightarrow> bool" where 
+"inc_index_inv2 e \<equiv> dnfp_precondition e
+                      \<and> invariant_low_to_j_is_1_Env e"
+
+definition inc_index_inv2_aux:: "env \<Rightarrow> bool" where
+"inc_index_inv2_aux e \<equiv> inc_index_inv2 e \<and> \<not>(xs e)!(i e) > 1 \<and> \<not>(xs e)!(i e) < 1 \<and> loop_update_action_pre e"         
+
+definition inc_index_inv3:: "env \<Rightarrow> bool" where
+"inc_index_inv3 e \<equiv> dnfp_precondition e
+                    \<and> high_invariant_is_2_Env e"
+
+definition inc_index_inv3_aux:: "env \<Rightarrow> bool" where
+"inc_index_inv3_aux e \<equiv> inc_index_inv3 e \<and> \<not>(xs e)!(i e) > 1 \<and> \<not>(xs e)!(i e) < 1 \<and> loop_update_action_pre e"
+
+definition inc_index_inv :: "env \<Rightarrow> bool" where
+"inc_index_inv s \<equiv> (inc_index_inv3 s \<and> inc_index_inv2 s \<and> inc_index_inv1 s)"
+
+definition inc_index_inv_aux:: "env \<Rightarrow> bool" where
+"inc_index_inv_aux e \<equiv> inc_index_inv e \<and> \<not>(xs e)!(i e) > 1 \<and> \<not>(xs e)!(i e) < 1 \<and> loop_update_action_pre e"
+
+
 
 definition dnfp_inv1:: "env \<Rightarrow> bool" where 
 "dnfp_inv1  e \<equiv> dnfp_precondition e
@@ -255,5 +306,15 @@ definition dnfp_inv2:: "env \<Rightarrow> bool" where
 definition dnfp_inv3:: "env \<Rightarrow> bool" where
 "dnfp_inv3 e \<equiv> dnfp_precondition e
                 \<and> high_invariant_is_2_Env e"
+
+definition dnfp_mon_inv :: "env \<Rightarrow> bool" where
+"dnfp_mon_inv e \<equiv> ((dnfp_inv3 e) \<and> (dnfp_inv2 e) \<and> (dnfp_inv1 e))"
+
+definition dnfp_post_final_spec where
+"dnfp_post_final_spec e \<equiv> dnfp_mon_inv e \<and> i e = high e"
+
+definition dnfp_mon_spec where
+"dnfp_mon_spec e \<equiv> dnfp_precondition e
+                    \<and> dnfp_mon_inv e"
 
 end
