Monad_Play Around/DNFP/Dutch_National_Flag_Monad_Eisbach.thy
@@ -1,0 +1,24 @@
+theory Dutch_National_Flag_Monad_Eisbach
+imports 
+  "Dutch_National_Flag_Monad_Definitions"
+  "HOL-Eisbach.Eisbach"
+begin
+
+method rewrite_env uses simps =
+(match conclusion in "?P (x :: env)" for x \<Rightarrow>
+  \<open>simp add: spec_def put_def get_state_def put_state_def return_def get_def simps\<close>)
+
+method rewrite_env_all =
+(match conclusion in "?P (x :: env)" for x \<Rightarrow>
+  \<open>simp add: spec_def put_def get_state_def put_state_def return_def get_def high_Env_def i_Env_def low_Env_def xs_Env_def swap_def\<close>)
+
+method all_Get_Seq =
+(intro allI; simp; intro get_rule; intro allI)
+
+method solve methods m = (m ; fail)
+
+method prop_solver =
+(rewrite_env_all; solve\<open>prop_solver\<close> | all_Get_Seq;  solve\<open>prop_solver\<close> )
+
+
+end
